cook a bogstandard brew

HOL_To_IMP_Minus/Refinements/HOL_To_IMP_Minus_Datatypes.thy
@@ -6,46 +6,88 @@ theory HOL_To_IMP_Minus_Datatypes
 begin
 
 datatype_compile_nat cmp_val
+datatype 'a my_option = None | Some 'a
+datatype_compile_nat my_option
+(* datatype_compile_nat option *) (* ?? *)
 
 locale HOL_To_HOL_Nat =
   notes transport_eq_id.partial_equivalence_rel_equivalenceI[per_intro del]
   and transport_eq_restrict_id.partial_equivalence_rel_equivalence[per_intro del]
 begin
 
-section \<open>Pairs\<close>
+
+section \<open>Pair\<close>
 
 function_compile_nat fst_def
 function_compile_nat snd_def
 
+
 section\<open>Three-way compare\<close>
 
+(* would require ord typeclass *)
 (* function_compile_nat cmp_def *)
 
-section\<open>Lists\<close>
+
+section\<open>Comparison (nat)\<close>
+
+fun "leq_aux" :: "nat \<Rightarrow> nat \<Rightarrow> bool" where
+  "leq_aux 0 _ = True" |
+  "leq_aux (Suc _) 0 = False" |
+  "leq_aux (Suc x) (Suc y) = leq_aux x y"
+
+lemma leq_eq_leq_aux: "(x \<le> y) \<equiv> leq_aux x y"
+  by (induction x y rule: leq_aux.induct) auto
+
+case_of_simps leq_aux_eq : leq_aux.simps
+function_compile_nat leq_aux_eq
+function_compile_nat leq_eq_leq_aux
+
+
+section \<open>Option\<close>
+
+paragraph \<open>is_some\<close>
+
+fun is_some :: "'a my_option \<Rightarrow> bool" where
+  "is_some (Some _) = True" |
+  "is_some None = False"
+
+case_of_simps is_some_eq : is_some.simps
+function_compile_nat is_some_eq
+
+
+paragraph \<open>get_some\<close>
+
+fun get_some :: "'a \<Rightarrow> 'a my_option \<Rightarrow> 'a" where
+  "get_some _ (Some x) = x" |
+  "get_some d _ = d"
+
+case_of_simps get_some_eq : get_some.simps
+function_compile_nat get_some_eq
+
+
+section\<open>List\<close>
 
 paragraph \<open>length\<close>
 
-(*
 fun length_aux :: "nat \<Rightarrow> 'a list \<Rightarrow> nat" where
   "length_aux acc [] = acc" |
   "length_aux acc (_ # xs) = length_aux (Suc acc) xs"
 
+(* definition length0 :: "'a list \<Rightarrow> nat" where *)
+  (* "length0 = length_aux 0" *)
 
-fun length :: "'a list \<Rightarrow> nat" where
-  "length [] = 0" |
-  "length (_ # xs) = Suc (length xs)"
+lemma length_eq_length_aux: "List.length xs + k = length_aux k xs"
+  by (induction k xs rule: length_aux.induct) auto
 
-lemma "List.length xs = local.length xs" by (induction xs) auto
+lemma length_eq_length0: "List.length xs = length_aux 0 xs"
+  (* unfolding length0_def *)
+  by (rule length_eq_length_aux[where k = 0, simplified])
 
-case_of_simps length_eq : length.simps
-function_compile_nat length_eq
-*)
+case_of_simps length_aux_eq : length_aux.simps
+function_compile_nat length_aux_eq
+(* function_compile_nat length0_def *)
+function_compile_nat length_eq_length0
 
-lemma length_eq: "length xs = (case xs of [] \<Rightarrow> 0 | (_ # xs') \<Rightarrow> Suc (length xs'))"
-  by (simp add: list.case_eq_if)
-
-function_compile_nat length_eq
-print_theorems
 
 paragraph\<open>compare_lengths\<close>
 
@@ -56,36 +98,158 @@ fun compare_lengths :: "'a list \<Rightarrow> 'b list \<Rightarrow> cmp_val" whe
   "compare_lengths (_ # xs) (_ # ys) = compare_lengths xs ys"
 
 case_of_simps compare_lengths_eq : compare_lengths.simps
-
 function_compile_nat compare_lengths_eq
+
+
+paragraph \<open>rev_append\<close>
+
+fun rev_append :: "'a list \<Rightarrow> 'a list \<Rightarrow> 'a list" where
+  "rev_append [] acc = acc" |
+  "rev_append (x # xs) acc = rev_append xs (x # acc)"
+
+case_of_simps rev_append_eq : rev_append.simps
+function_compile_nat rev_append_eq
+
 
 paragraph \<open>rev\<close>
 
-fun rev_aux :: "'a list \<Rightarrow> 'a list \<Rightarrow> 'a list" where
-  "rev_aux acc [] = acc" |
-  "rev_aux acc (x # xs) = rev_aux (x # acc) xs"
+definition rev0 :: "'a list \<Rightarrow> 'a list" where
+  "rev0 xs = rev_append xs []"
 
-case_of_simps rev_aux_eq : rev_aux.simps
+lemma rev_eq_rev_aux: "List.rev xs @ ys = local.rev_append xs ys"
+  by (induction xs ys rule: rev_append.induct) auto
 
-function_compile_nat rev_aux_eq
+lemma rev_eq_rev0: "List.rev xs = local.rev0 xs"
+  unfolding rev0_def
+  using rev_eq_rev_aux[where ys = "[]"] by simp
 
-definition rev :: "'a list \<Rightarrow> 'a list" where
-  "rev = rev_aux []"
+function_compile_nat rev0_def
+function_compile_nat rev_eq_rev0
 
-function_compile_nat rev_def
+
+paragraph \<open>append\<close>
+
+lemma append_eq_append0: "List.append xs ys = rev_append (rev xs) ys"
+  unfolding rev_eq_rev_aux[symmetric] by simp
+
+function_compile_nat append_eq_append0
+
 
 paragraph \<open>zip\<close>
 
-thm zip.simps
-case_of_simps zip_eq : zip.simps
-function_compile_nat zip_eq
+fun zip_aux :: "('a \<times> 'b) list \<Rightarrow> 'a list \<Rightarrow> 'b list \<Rightarrow> ('a \<times> 'b) list" where
+  "zip_aux acc [] _ = acc" |
+  "zip_aux acc _ [] = acc" |
+  "zip_aux acc (x # xs) (y # ys) = zip_aux ((x, y) # acc) xs ys"
+
+lemma zip_eq_zip_aux: "rev zs @ List.zip xs ys = rev (zip_aux zs xs ys)"
+  apply (induction zs xs ys rule: zip_aux.induct)
+  unfolding rev_eq_rev0[symmetric] by auto
+
+lemma zip_eq_zip_aux0: "List.zip xs ys = rev (zip_aux [] xs ys)"
+  using zip_eq_zip_aux[where zs = "[]"]
+  unfolding rev_eq_rev0[symmetric] by auto
+
+case_of_simps zip_aux_eq : zip_aux.simps
+function_compile_nat zip_aux_eq
+function_compile_nat zip_eq_zip_aux0 (* slow? *)
+
+
+subsection \<open>Association Lists\<close>
+
+fun assoc_lookup :: "'k \<Rightarrow> ('k \<times> 'v) list \<Rightarrow> 'v my_option" where
+  "assoc_lookup _ [] = None" |
+  "assoc_lookup x ((k, v) # xs) = (if x = k then Some v else assoc_lookup k xs)"
+
+case_of_simps assoc_lookup_eq : assoc_lookup.simps
+function_compile_nat assoc_lookup_eq
+
+(* TODO: assoc_delete, assoc_update *)
+
+subsection \<open>Sorting\<close>
+
+text \<open>Sorting, based on decorate-sort-undecorate. Sorts tuples (nat, 'a) on the nat component.
+  For sorting arbitrary datatypes, they must first be mapped to an integer key, sorted, then
+  the key stripped away. Best we can do, since we cannot write a polymorphic sort.\<close>
+(* TODO: or can we do something with typeclasses? *)
+
+type_synonym 'a sort_key = "(nat \<times> 'a)"
+
+fun insort_deco_aux :: "'a sort_key list \<Rightarrow> 'a sort_key \<Rightarrow> 'a sort_key list \<Rightarrow> 'a sort_key list" where
+  "insort_deco_aux acc k [] = rev (k # acc)" |
+  "insort_deco_aux acc k' (k # xs) =
+    (if fst k' \<le> fst k then rev_append (k' # acc) (k # xs) else insort_deco_aux (k # acc) k' xs)"
+
+case_of_simps insort_deco_aux_eq : insort_deco_aux.simps
+(* function_compile_nat insort_deco_aux_eq *)
+(* this refuses to compile *)
+
+lemma insort_key_fst_eq_insort_deco_aux: "rev acc @ insort_key fst k xs = insort_deco_aux acc k xs"
+  apply (induction acc k xs rule: insort_deco_aux.induct) using rev_eq_rev_aux by auto
+
+definition insort_deco :: "'a sort_key \<Rightarrow> 'a sort_key list \<Rightarrow> 'a sort_key list" where
+  "insort_deco = insort_deco_aux []"
+
+lemma insort_key_fst_eq_insort_deco_aux0: "insort_key fst k xs = insort_deco k xs"
+  unfolding insort_deco_def using insort_key_fst_eq_insort_deco_aux[where acc = "[]", simplified] by fast
+
+(* function_compile_nat insort_deco_def *)
+
+fun sort_deco_aux :: "'a sort_key list \<Rightarrow> 'a sort_key list \<Rightarrow> 'a sort_key list" where
+  "sort_deco_aux acc [] = acc" |
+  "sort_deco_aux acc (x # xs) = sort_deco_aux (insort_deco x acc) xs"
+
+case_of_simps sort_deco_aux_eq : sort_deco_aux.simps
+(* function_compile_nat sort_deco_aux_eq *)
+
+lemma sort_key_eq_sort_deco_aux:
+  assumes sorted_acc: "sorted (map fst acc)" shows "sort_key fst (xs @ acc) = sort_deco_aux acc (rev xs)"
+proof-
+  have "sort_key fst (xs @ acc) = foldl (\<lambda>x y. insort_key fst y x) acc (rev xs)"
+    by (subst sort_key_def, subst foldr_append, subst sort_key_def[symmetric],
+        subst sort_key_id_if_sorted[OF sorted_acc], subst foldr_conv_foldl, rule refl)
+  moreover have "foldl (\<lambda>x y. insort_key fst y x) acc xs = sort_deco_aux acc xs" for xs
+    by (induction xs arbitrary: acc) (auto simp add: insort_key_fst_eq_insort_deco_aux0)
+  ultimately show "sort_key fst (xs @ acc) = sort_deco_aux acc (rev xs)" by simp
+qed
+
+lemma sort_key_eq_sort_deco_aux0: "sort_key fst xs = sort_deco_aux [] (rev xs)"
+  using sort_key_eq_sort_deco_aux[where acc = "[]"] by auto
+
+definition sort_deco :: "'a sort_key list \<Rightarrow> 'a sort_key list" where
+  "sort_deco = sort_deco_aux []"
+
+(* function_compile_nat sort_deco_def *)
+
+(* For sort_deco and helpers it's not really clear how to generate a "drop-in" compilable function
+   compatible with sort, since we can't compile "sort_key fst" to IMP. Thus, code will
+   need to call sort_deco directly (but the correctness lemmas should still be useful). *)
+
+fun undecorate_aux :: "'a list \<Rightarrow> 'a sort_key list \<Rightarrow> 'a list" where
+  "undecorate_aux acc [] = rev acc" | "undecorate_aux acc ((_, x) # xs) = undecorate_aux (x # acc) xs"
+
+definition undecorate :: "'a sort_key list \<Rightarrow> 'a list" where
+  "undecorate = undecorate_aux []"
+
+case_of_simps undecorate_aux_eq : undecorate_aux.simps
+function_compile_nat undecorate_aux_eq
+function_compile_nat undecorate_def
 
 end
 
 context HOL_To_IMP_Minus
 begin
 
-section \<open>Pairs\<close>
+section \<open>Bool\<close>
+
+compile_nat True_nat_def
+HOL_To_IMP_Minus_correct True_nat by cook
+
+compile_nat False_nat_def
+HOL_To_IMP_Minus_correct False_nat by cook
+
+
+section \<open>Pair\<close>
 
 compile_nat Pair_nat_def
 HOL_To_IMP_Minus_correct Pair_nat by cook
@@ -100,6 +264,7 @@ unconditional_nat snd_nat_eq_unfolded
 compile_nat snd_nat_unconditional.simps
 HOL_To_IMP_Minus_correct snd_nat_unconditional by cook
 
+
 section \<open>Three-way compare\<close>
 
 compile_nat LT_nat_def
@@ -111,6 +276,50 @@ HOL_To_IMP_Minus_correct EQ_nat by cook
 compile_nat GT_nat_def
 HOL_To_IMP_Minus_correct GT_nat by cook
 
+
+section\<open>Comparison (nat)\<close>
+
+find_theorems "case (?x :: nat) of (0) \<Rightarrow> _ | (Suc n) \<Rightarrow> _" "if ?x = 0 then _ else _"
+
+lemmas leq_aux_nat_eq = HOL_To_HOL_Nat.leq_aux_nat_eq_unfolded[simplified case_nat_eq_if]
+unconditional_nat leq_aux_nat_eq
+declare leq_aux_nat_unconditional.simps [simp del]
+compile_nat leq_aux_nat_unconditional.simps
+HOL_To_IMP_Minus_correct leq_aux_nat_unconditional by (cook mode = tailcall)
+
+unconditional_nat HOL_To_HOL_Nat.leq_eq_leq_aux
+declare less_eq_unconditional.simps [simp del]
+(* TODO: uses helper function *)
+(* compile_nat less_eq_unconditional.simps *)
+(* HOL_To_IMP_Minus_correct less_eq_unconditional by cook *)
+
+
+section \<open>Option\<close>
+
+compile_nat None_nat_def
+HOL_To_IMP_Minus_correct None_nat by cook
+
+compile_nat Some_nat_def
+HOL_To_IMP_Minus_correct Some_nat by cook
+
+
+paragraph \<open>is_some\<close>
+
+lemmas is_some_nat_eq = HOL_To_HOL_Nat.is_some_nat_eq_unfolded[simplified case_my_option_nat_def]
+unconditional_nat is_some_nat_eq
+declare is_some_nat_unconditional.simps [simp del]
+compile_nat is_some_nat_unconditional.simps
+HOL_To_IMP_Minus_correct is_some_nat_unconditional by cook
+
+paragraph \<open>get_some\<close>
+
+lemmas get_some_nat_eq = HOL_To_HOL_Nat.get_some_nat_eq_unfolded[simplified case_my_option_nat_def]
+unconditional_nat get_some_nat_eq
+declare get_some_nat_unconditional.simps [simp del]
+compile_nat get_some_nat_unconditional.simps
+HOL_To_IMP_Minus_correct get_some_nat_unconditional by cook
+
+
 section\<open>Lists\<close>
 
 compile_nat Cons_nat_def
@@ -121,15 +330,20 @@ HOL_To_IMP_Minus_correct Nil_nat by cook
 
 paragraph \<open>length\<close>
 
-(* TODO: these all end up getting named size_... *)
-thm HOL_To_HOL_Nat.size_nat_eq_unfolded
-lemmas size_nat_eq = HOL_To_HOL_Nat.size_nat_eq_unfolded[simplified case_list_nat_def]
-unconditional_nat size_nat_eq basename length_nat
-declare length_nat_unconditional.simps [simp del]
-compile_nat length_nat_unconditional.simps
-print_theorems
-(* TODO: also the proof doesn't work *)
-(* HOL_To_IMP_Minus_correct length_nat_unconditional by (cook mode = tailcall) *)
+lemmas length_aux_nat_eq = HOL_To_HOL_Nat.length_aux_nat_eq_unfolded[simplified case_list_nat_def]
+unconditional_nat length_aux_nat_eq
+declare length_aux_nat_unconditional.simps [simp del]
+compile_nat length_aux_nat_unconditional.simps
+HOL_To_IMP_Minus_correct length_aux_nat_unconditional by (cook mode = tailcall)
+
+(* TODO: this ends up getting named size_... *)
+lemmas length_nat_eq = HOL_To_HOL_Nat.size_nat_eq_unfolded[simplified case_list_nat_def]
+(* TODO: uses helper function *)
+(* unconditional_nat length_nat_eq *)
+(* declare length_nat_unconditional.simps [simp del] *)
+(* compile_nat length_nat_unconditional.simps *)
+(* HOL_To_IMP_Minus_correct length_nat_unconditional by cook *)
+
 
 paragraph\<open>compare_lengths\<close>
 
@@ -139,29 +353,49 @@ declare compare_lengths_nat_unconditional.simps [simp del]
 compile_nat compare_lengths_nat_unconditional.simps
 HOL_To_IMP_Minus_correct compare_lengths_nat_unconditional by (cook mode = tailcall)
 
+
+paragraph \<open>rev_append\<close>
+
+lemmas rev_append_nat_eq = HOL_To_HOL_Nat.rev_append_nat_eq_unfolded[simplified case_list_nat_def]
+unconditional_nat rev_append_nat_eq
+declare rev_append_nat_unconditional.simps [simp del]
+compile_nat rev_append_nat_unconditional.simps
+HOL_To_IMP_Minus_correct rev_append_nat_unconditional by (cook mode = tailcall)
+
 paragraph \<open>rev\<close>
 
-lemmas rev_aux_nat_eq = HOL_To_HOL_Nat.rev_aux_nat_eq_unfolded[simplified case_list_nat_def]
-unconditional_nat rev_aux_nat_eq
-declare rev_aux_nat_unconditional.simps [simp del]
-compile_nat rev_aux_nat_unconditional.simps
-HOL_To_IMP_Minus_correct rev_aux_nat_unconditional by (cook mode = tailcall)
+(* TODO: can't do functions with helpers! *)
 
-(*
-TODO: can't do functions with helpers!
-thm HOL_To_HOL_Nat.rev_nat_eq_unfolded
-lemmas rev_nat_eq = HOL_To_HOL_Nat.rev_nat_eq_unfolded[simplified case_list_nat_def]
-unconditional_nat rev_nat_eq
-*)
+
+paragraph \<open>append\<close>
+
+(* TODO: aux function *)
+
 
 paragraph \<open>zip\<close>
 
-lemmas zip_nat_eq = HOL_To_HOL_Nat.zip_nat_eq_unfolded[simplified case_list_nat_def]
-unconditional_nat zip_nat_eq
-declare zip_nat_unconditional.simps [simp del]
-compile_nat zip_nat_unconditional.simps
-(* TODO: proof fails *)
-(* HOL_To_IMP_Minus_correct zip_nat_unconditional by (cook mode = tailcall) *)
+lemmas zip_aux_nat_eq = HOL_To_HOL_Nat.zip_aux_nat_eq_unfolded[simplified case_list_nat_def]
+unconditional_nat zip_aux_nat_eq
+declare zip_aux_nat_unconditional.simps [simp del]
+compile_nat zip_aux_nat_unconditional.simps
+HOL_To_IMP_Minus_correct zip_aux_nat_unconditional by (cook mode = tailcall)
+
+(* TODO: zip: aux function needed *)
+
+
+subsection \<open>Association Lists\<close>
+
+lemmas assoc_lookup_nat_eq = HOL_To_HOL_Nat.assoc_lookup_nat_eq_unfolded[simplified case_list_nat_def case_prod_nat_def]
+unconditional_nat assoc_lookup_nat_eq
+declare assoc_lookup_nat_unconditional.simps [simp del]
+compile_nat assoc_lookup_nat_unconditional.simps
+HOL_To_IMP_Minus_correct assoc_lookup_nat_unconditional by (cook mode = tailcall)
+
+
+subsection \<open>Sorting\<close>
+
+(* TODO: get compiling to Nat first *)
+
 
 end
 
